# 3.2 Standard notations and common functions
## 3.2-1
If f(n) and g(n) are monotonically increasing functions, then if $m \leq n$, we have $f(m) \leq f(n)$ and $g(m) \leq g(n)$. So we get $f(m) + g(m) \leq f(n) + g(n)$ when $m \leq n$. So the function f(n) + g(n) is monotonically increasing.

Let $m_1 = g(m)$ and $n_1 = g(n)$. Because $m_1 \leq n_1$, so $f(m_1) \leq f(n_1)$, so f(g(n)) is monotonically increasing.

if f(n) and g(n) are nonnegative, because $f(m) \leq f(n)$ and $g(m) \leq g(n)$, so we can multiply the inequations and have $f(m) \cdot g(m) \leq f(n) \cdot g(n)$. Thus $f(n) \cdot g(n)$ is monotonically increasing.

## 3.2-2
$a^{\log_bc} = a^{\frac{\log_ac}{\log_ab}} = (a^{\log_ac})^\frac{1}{\log_ab} = c^\frac{1}{\log_ab} = c^{\log_ba}$.

## 3.2-3
According to [Stirling's approximation](https://en.wikipedia.org/wiki/Stirling%27s_approximation), we have:

$$\sqrt{2\pi}n^{n + \frac{1}{2}}e^{-n} \leq n! \leq en^{n + \frac{1}{2}}e^{-n}$$

So:

$$\lg{(\sqrt{2\pi}n^{n + \frac{1}{2}}e^{-n})} \leq \lg{(n!)} \leq \lg{(en^{n + \frac{1}{2}}e^{-n})}$$

Notice that:

$$
\begin{eqnarray}
\lg{(\sqrt{2\pi}n^{n + \frac{1}{2}}e^{-n})} &=& \lg{(\sqrt{2\pi})} + \lg{n^{n + \frac{1}{2}}} + \lg{e^{-n}} \\\
&=& \lg{(\sqrt{2\pi})} + (n + \frac{1}{2})\lg{n} - n\lg{e} \\\
&=& n(\lg{n} - \lg{e}) + \lg{(\sqrt{2\pi})} + \frac{1}{2}\lg{n} \\\
&\geq& n(\lg{n} - \lg{\sqrt{n}}) + \lg{(\sqrt{2\pi})} + \frac{1}{2}\lg{n} \text{ (when } n \geq e^2 \text{)} \\\
&=& n\lg{\frac{n}{\sqrt{n}}} + \lg{(\sqrt{2\pi})} + \frac{1}{2}\lg{n} \\\
&=& \frac{1}{2}n\lg{n} + \lg{(\sqrt{2\pi})} + \frac{1}{2}\lg{n} \\\
&\geq& \frac{1}{2}n\lg{n}
\end{eqnarray}
$$

And:

$$
\begin{eqnarray}
\lg{(en^{n + \frac{1}{2}}e^{-n})} &=& \lg{e} + \lg{n^{n + \frac{1}{2}}} + \lg{e^{-n}} \\\
&=& \lg{e} + (n + \frac{1}{2})\lg{n} + \lg{e^{-n}} \\\
&=& n\lg{n} + \lg{e} + \frac{1}{2}\lg{n} + \lg{e^{-n}} \\\
&=& n\lg{n} + \lg{\frac{e\sqrt{n}}{e^n}} \\\
&\leq& n\lg{n} + \lg{1} \text{ (when } n \geq 1 \text{)} \\\
&=& n\lg{n}
\end{eqnarray}
$$

So now we get:

$$\frac{1}{2}n\lg{n} \leq \lg{(n!)} \leq n\lg{n} \text{ (when } n \geq e^2 \text{)}$$

which means: there exist positive constants $c_1 = \frac{1}{2}$, $c_2 = 1$ and $n_0 = 8$ such that:

$$0 \leq c_1n\lg{n} \leq \lg(n!) \leq c_2n\lg{n},\ for \ all \ n \geq n_0$$

So $\lg{(n!)} = \Theta(n\lg{n})$.

When $n \geq 4$, we have:

$$
\begin{eqnarray}
n! &=& n * (n - 1) * \ldots * 4 * 3 * 2 * 1 \\\
&=& n * (n - 1) * \ldots * 2 * 2 * 3 * 2 * 1 \\\
&>& 2 * 2 * \ldots * 2 * 2 * 3 * 2 * 1 \\\
&=&  2^n * 1 \\\
&=& 2^n
\end{eqnarray}
$$

So for any positive constant $c_1$, there exist positive constant $n_1 = 4$, such that $0 \leq c_1(2^n) < n! \ for\ all\ n \geq n_1$.

So $n! = w(2^n)$.

When $n \geq 2$, we have:

$$
\begin{eqnarray}
n! &=& n * (n - 1) * \ldots * 2 * 1 \\\
&<& n * n * \ldots * n * n \\\
&=&  n^n
\end{eqnarray}
$$

So for any positive constant $c_2$, there exist positive constant $n_2 = 2$, such that $0 \leq n! < c_2n^n \ for\ all\ n \geq n_2$.

So $n! = o(n^n)$.

## 3.2-4
Suppose $\lceil \lg{n} \rceil!$ is polynomially bounded, then there exist positive constants c, k and $n_0$ such that $0 \leq \lceil \lg{n} \rceil! \leq cn^k$ for all $n \geq n_0$. So $\lg{(\lceil \lg{n} \rceil!)} \leq \lg{(cn^k)}$.

But:

$$
\begin{eqnarray}
\lg{(\lceil \lg{n} \rceil!)} - \lg{(cn^k)} &\geq& \lg{((\lg{n})!)} - \lg{(cn^k)} \\\
&\geq& \frac{1}{2}\lg{n} * \lg{(\lg{n})} - \lg{(cn^k)} \text{ (reuse the inequation in 3.2-3)} \\\
&=& \frac{1}{2}\lg{n} * \lg{(\lg{n})} - \lg{c} - k\lg{n} \\\
&=& \lg{n}(\frac{1}{2}\lg{(\lg{n})} - k) - \lg{c}
\end{eqnarray}
$$

Since both k and c are constants and $\lg{n}$ is a monotonically increasing function, it's obvious that there exist positive constants $n_1$ and $n_2$ such that $\frac{1}{2}\lg{(\lg{n})} - k \geq 0 \text{ for all } n \geq n_1$ and $b\lg{n} - \lg{c} \geq 0, b = \frac{1}{2}\lg{(\lg{n})} - k \geq 0 \text{ for all } n \geq n_2$. So we can let $n_3 = max(n_1, n_2)$ such that $\lg{(\lceil \lg{n} \rceil!)} - \lg{(cn^k)} \geq 0 \text{ for all } n \geq n_3$.

So we know that the hypothesis is not correct, thus $\lceil \lg{n} \rceil!$ is not polynomially bounded.

Now let's prove that $\lceil \lg{\lg{n}} \rceil!$ is polynomially bounded.

$$
\begin{eqnarray}
\lg{(\lceil \lg{\lg{n}} \rceil!)} - \lg{(cn^k)} &\leq& \lceil \lg{\lg{n}} \rceil\lg{(\lceil \lg{\lg{n}} \rceil)} - \lg{(cn^k)} \text{ (reuse the inequation in 3.2-3)} \\\
&=& \lceil \lg{\lg{n}} \rceil\lg{(\lceil \lg{\lg{n}} \rceil)} - \lg{c} - k\lg{n} \\\
&<& (\lg{\lg{n}} + 1)\lg{(\lg{\lg{n}} + 1)} - \lg{c} - k\lg{n} \\\
\end{eqnarray}
$$

Let $\lg{n} = x, x > 0$, so $(\lg{\lg{n}} + 1)\lg{(\lg{\lg{n}} + 1)} - \lg{c} - k\lg{n} = (\lg{x} + 1)\lg{(\lg{x} + 1)} - \lg{c} - kx = f(x)$.

So $f'(x) = \frac{\lg{(\lg{x} + 1)} + 1}{x} - k$.

Let $g(x) = \frac{\lg{(\lg{x} + 1)} + 1}{x}$, so $g'(x) = \frac{\frac{1}{\lg{x} + 1} - (\lg{(\lg{x} + 1)} + 1)}{x^2}$. It's easy to see that g'(x) is a monotonically decreasing function and g'(1) = 0, so $g(x) \leq 0 \text{ on } [1, +\infty)$. So g(x) is monotonically decreasing on $[1, +\infty)$ and g(1) = 1.

So $f'(x) \leq 1 - k \text{ on } [1, +\infty)$. And for some constants k, $f'(x) \leq 0$. Thus f(x) is also a monotonically decreasing function on $[1, +\infty)$ for some constants k. And $f(1) = -\lg{c} - k < 0$, so f(x) < 0 on $[1, +\infty)$.

So there exist positive constants c, k and $n_0 = 2$ such that $\lg{(\lceil \lg{\lg{n}} \rceil!)} - \lg{(cn^k)} < f(x) < 0 \text{ for all } n \geq n_0$. So $\lceil \lg{\lg{n}} \rceil! \leq cn^k$. So $\lceil \lg{\lg{n}} \rceil!$ is polynomially bounded.

## 3.2-5
[Here](https://en.wikipedia.org/wiki/Iterated_logarithm) is the definition of $\lg^\*{n}$. So $\lg{(\lg^\*{n})} = \lg{(1 + \lg^\*{(\lg{n})})}$. Let $\lg^\*{(\lg{n})} = x$, so it's obvious $f(x) = \lg{(1 + x)}$ grows slower than $g(x) = x$, so $\lg^\*{(\lg{n})}$ is asymptotically larger.

## 3.2-6
$$
\begin{eqnarray}
\phi^2 - \phi - 1 &=& (\frac{1 + \sqrt{5}}{2})^2 - \frac{1 + \sqrt{5}}{2} - 1 \\\
&=& \frac{1 + 2\sqrt{5} + 5}{4} - \frac{2 + 2\sqrt{5}}{4} - \frac{4}{4} \\\
&=& \frac{6 + 2\sqrt{5} - 2 - 2\sqrt{5} - 4}{4} \\\
&=& 0
\end{eqnarray}
$$

$$
\begin{eqnarray}
\hat\phi^2 - \hat\phi - 1 &=& (\frac{1 - \sqrt{5}}{2})^2 - \frac{1 - \sqrt{5}}{2} - 1 \\\
&=& \frac{1 - 2\sqrt{5} + 5}{4} - \frac{2 - 2\sqrt{5}}{4} - \frac{4}{4} \\\
&=& \frac{6 - 2\sqrt{5} - 2 + 2\sqrt{5} - 4}{4} \\\
&=& 0
\end{eqnarray}
$$

So the golden ratio $\phi$ and its conjugate $\hat\phi$ both satisfy the equation $x^2 = x + 1$.

## 3.2-7
