# 4.4 The recursion-tree method for solving recurrences
## 4.4-1
First let's create a recursion tree for the recurrence $T(n) = 3T(\frac{n}{2}) + n$ and assume that n is an exact power of 2.

```
\documentclass{standalone} 
\usepackage{tikz}
\usetikzlibrary{positioning}

\tikzset{
    no edge from this parent/.style={
        every child/.append style={
        edge from parent/.style={draw=none}}},
    level 4/.style={level distance=6mm} 
}

\begin{document}
\begin{tikzpicture}
\tikzstyle{level 1}=[sibling distance=24mm]
\tikzstyle{level 2}=[sibling distance=8mm]
\tikzstyle{level 3}=[sibling distance=4mm]

\node (root){n} 
    child {node {$\frac{n}{2}$}
        child {node {$\frac{n}{4}$}
            child{node {$\vdots$}[no edge from this parent]
                child{node {T(1)}}}}
        child {node {$\frac{n}{4}$}
            child{node {$\vdots$}[no edge from this parent]
                child{node {T(1)}}}}
        child {node {$\frac{n}{4}$}
            child{node {$\vdots$}[no edge from this parent]
                child{node {T(1)}}}}}
    child {node {$\frac{n}{2}$}
        child {node {$\frac{n}{4}$}
            child{node {$\vdots$}[no edge from this parent]
                child{node {T(1)}}}}
        child {node {$\frac{n}{4}$}
            child{node {$\vdots$}[no edge from this parent]
                child{node {T(1)}}}}
        child {node {$\frac{n}{4}$}
            child{node {$\vdots$}[no edge from this parent]
                child{node {T(1)}}}}}
    child {node {$\frac{n}{2}$}
        child {node {$\frac{n}{4}$}
            child{node {$\vdots$}[no edge from this parent]
                child{node {T(1)}}}}
        child {node {$\frac{n}{4}$}
            child{node {$\vdots$}[no edge from this parent]
                child{node {T(1)}}}}
        child {node {$\frac{n}{4}$}
            child{node {$\vdots$}[no edge from this parent]
                child{node {T(1)}}}}};

\node[right=4 of root] {n}[no edge from this parent]
    child {node {$\frac{3n}{2}$}[no edge from this parent]
        child {node {$(\frac{3}{2})^2n$}[no edge from this parent]
            child {node {}[no edge from this parent]
                child {node {$\Theta(n^{\lg{3}})$}}}}};
\end{tikzpicture}
\end{document}
```

![Alt text](4.4-1.png)

Each level has three times more nodes than the level above, so the number of nodes at depth i is $3^i$. And each node at depth i, for $i = 0, 1, 2, \ldots, \lg{n} - 1$, has a cost of $\frac{n}{2^i}$. So the total cost over all nodes at depth i, is $3^i\frac{n}{2^i} = (\frac{3}{2})^in$. The bottom level, at depth $\lg{n}$, has $3^{\lg{n}} = n^{\lg{3}}$ nodes, each contributing cost $T(1)$, for a total cost of $n^{\lg{3}}T(1)$, which is $\Theta(n^{\lg{3}})$. So:

$$
\begin{eqnarray}
T(n) &=& \sum_{i = 0}^{\lg{n} - 1}(\frac{3}{2})^in + \Theta(n^{\lg{3}}) \\\
&=& n\frac{1 - (\frac{3}{2})^{\lg{n}}}{1 - \frac{3}{2}} + \Theta(n^{\lg3}) \\\
&=& 2n\frac{3^{\lg{n}} - 2^{\lg{n}}}{2^{\lg{n}}} + \Theta(n^{\lg3}) \\\
&=& 2n\frac{3^{\lg{n}} - 2^{\lg{n}}}{n} + \Theta(n^{\lg3}) \\\
&=& 2(3^{\lg{n}} - 2^{\lg{n}}) + \Theta(n^{\lg3}) \\\
&=& 2(n^{\lg{3}} -n) + \Theta(n^{\lg3}) \\\
&<& 2n^{\lg3} + \Theta(n^{\lg3}) \\\
&=& O(n^{\lg3})
\end{eqnarray}
$$

Thus, we have derived a guess of $T(n) = O(n^{\lg3})$ for our original recurrence. Now let's use the substitution method to verify that our guess was correct. We want to show that $T(n) \leq cn^{\lg3}$ for some constant $c > 0$. So:

$$
\begin{eqnarray}
T(n) &=& 3T(\lfloor \frac{n}{2} \rfloor) + n \\\
&\leq& 3c\lfloor \frac{n}{2} \rfloor^{\lg3} + n \\\
&\leq& 3c(\frac{n}{2})^{\lg3} + n \\\
&=& 3c(\frac{n}{2})^{\lg3} + n \\\
&=& 3c\frac{n^{\lg3}}{2^{\lg3}} + n \\\
&=& 3c\frac{n^{\lg3}}{3} + n \\\
&=& cn^{\lg{3}} + n
\end{eqnarray}
$$

But $cn^{\lg{3}} + n > cn^{\lg{3}}$, so we need to try another guess. Let's try $T(n) \leq cn^{\lg3} - \frac{2n}{3}$. So:

$$
\begin{eqnarray}
T(n) &=& 3T(\lfloor \frac{n}{2} \rfloor) + n \\\
&\leq& 3(c\lfloor \frac{n}{2} \rfloor^{\lg3} - \frac{n}{3}) + n \\\
&\leq& 3(c(\frac{n}{2})^{\lg3} - \frac{n}{3}) + n \\\
&=& 3c(\frac{n}{2})^{\lg3} \\\
&=& cn^{\lg3}
\end{eqnarray}
$$

## 4.4-2