# 2.3 Designing algorithms
## 2.3-1
![Alt text](2.3-2.png)

## 2.3-2
```
MERGE(A, p, q, r)

n1 = q - p + 1
n2 = r - q
let L[1..n1] and R[1..n2] be new arrays
for i = 1 to n1
    L[i] = A[p + i - 1]
for j = 1 to n2
    R[j] = A[q + j]
i = 1
j = 1
for k = p to r
    if i > n1:
        A[k] = R[j]
        j = j + 1
    else if j > n2:
        A[k] = L[i]
        i = i + 1
    else if L[i] <= R[j]:
        A[k] = L[i]
        i = i + 1
    else
        A[k] = R[j]
        j = j + 1
```

## 2.3-3
Because n is an exact power of 2, so the sequence of n is $2, 4, 8, 16, \ldots, 2^k$. First, let's see the base case, the base case is $n = 2$. And we have $T(n) = 2 = 2\lg{2}$. So the statement holds true for $n = 2$.

Second, let's see the inductive step. We assume $T(n) = n\lg{n}$ is true when $n = 2^k, k > 1$, and we want to prove it also holds true for the $n + 1$ element, which is $2^{k + 1}$.

When $n = 2^{k + 1}$, we have:

$$
\begin{eqnarray}
T(2^{k + 1}) &=& 2T(\frac{2^{k + 1}}{2}) + 2^{k + 1} \\\\\\
&=& 2T(2^k) + 2^{k + 1} \\\\\\
&=& 2 * 2^k\lg{2^k} + 2^{k + 1} \\\\\\
&=& 2^{k + 1}\lg{2^k} + 2^{k + 1} \\\\\\
&=& 2^{k + 1}(\lg{2^k} + 1) \\\\\\
&=& 2^{k + 1}(\lg{2^k} + \lg{2}) \\\\\\
&=& 2^{k + 1}\lg{2^{k + 1}}
\end{eqnarray}
$$

So $T(n) = n\lg{n}$ is true for all $n = 2^k, k \geq 1$.
